theories/TypeSystem_Dataframe.v
@@ -1,0 +1,213 @@
+Set Warnings "-notation-overridden,-parsing".
+From Coq Require Import Lists.List.
+
+From DF Require Import Dataframe.
+
+(* Define terms. *)
+Inductive op : Type :=
+| DataFrame :
+   Dataframe.DataFrame -> op
+| Transpose : op -> op
+| Mask :
+    (** Mask positions. **) list nat ->
+    (** Axis to apply mask over **) Dataframe.Axis ->
+    op -> op
+| Filter :
+    (** Filter function **) (list Dataframe.data_value -> bool) ->
+    (** Axis to filter over **) Dataframe.Axis ->
+    op -> op
+| ToLabels :
+    (** Index to use as index labels **) nat ->
+    (** Axis to update the index for. **) Dataframe.Axis ->
+    op -> op
+| FromLabels :
+    (** Axis to take the index from. **) Dataframe.Axis ->
+    op -> op
+| Map :
+    (** Mapping function **) (list Dataframe.data_value -> list Dataframe.data_value) ->
+    (** Possible dtypes each index **) list (list Dataframe.dtype) ->
+    (** Axis to map over. **) Dataframe.Axis ->
+    op -> op
+| Concat :
+    (** How to concat **) Dataframe.Set_Combine ->
+    (** Axis to concat along. **) Dataframe.Axis ->    
+    (** Other dataframe to concat **) op ->
+    (** Self **) op ->
+    op
+| InferDTypes :
+    (** Axis to infer dtypes for. **) Dataframe.Axis ->
+    op -> op.
+
+(*
+Inductive dfvalue : op -> Prop :=
+| dfvalue_DataFrame : dfvalue DataFrame.
+ *)
+Inductive dfvalue : op -> Prop :=
+| df_DataFrame : forall df_obj,
+    (*
+    Datatypes.length row__index = Datatypes.length row__dtypes ->
+    Datatypes.length col__index = Datatypes.length col__dtypes ->
+    Dataframe.valid_matrix values = true ->
+    Dataframe.matrix_length values = Datatypes.length row__index ->
+    Dataframe.matrix_width values = Datatypes.length col__index ->
+    Dataframe.dtype_eqb_lsts (map infer_dtypes values) row__dtypes = true ->
+    Dataframe.dtype_eqb_lsts (map infer_dtypes (Dataframe.transpose_matrix values)) col__dtypes = true ->
+    Dataframe.valid_index row__index = true ->
+    Dataframe.valid_index col__index = true ->
+    dfvalue (DataFrame row__index row__dtypes col__index col__dtypes values).
+     *)
+    Dataframe.DataFrame -> dfvalue (DataFrame df_obj).
+
+Hint Constructors dfvalue : core.
+
+Reserved Notation "t '-->' t'" (at level 40).
+
+Inductive step : op -> op -> Prop :=
+| ST_TransposeValue : forall df df_obj,
+    dfvalue df ->
+    df = DataFrame df_obj ->
+    Transpose df --> DataFrame (Dataframe.Transpose df_obj)
+| ST_TransposeStep : forall df df',
+    df --> df' ->
+    Transpose df --> Transpose df'
+| ST_TransposeTwice : forall df,
+    dfvalue df ->
+    Transpose (Transpose df) --> df
+| ST_MaskValue : forall mask_position axis df df_obj,
+    dfvalue df ->
+    df = DataFrame df_obj ->
+    Mask mask_position axis df --> DataFrame (Dataframe.Mask mask_position axis df_obj)
+| ST_MaskStep : forall mask_position axis df df',
+    df --> df' ->
+    Mask mask_position axis df --> Mask mask_position axis df'
+(*
+| ST_FilterNone : forall axis df,
+    dfvalue df ->
+    Filter (fun row => true) axis df --> df
+ *)
+| ST_FilterValue : forall filter_func axis df df_obj,
+    dfvalue df ->
+    df = DataFrame df_obj ->
+    Filter filter_func axis df --> DataFrame (Dataframe.Filter filter_func axis df_obj)
+| ST_FilterStep : forall filter_func axis df df',
+    df --> df' ->
+    Filter filter_func axis df --> Filter filter_func axis df'
+| ST_ToLabelsValue : forall index_ind axis df df_obj,
+    dfvalue df ->
+    df = DataFrame df_obj ->
+    ToLabels index_ind axis df --> DataFrame (Dataframe.ToLabels index_ind axis df_obj)
+| ST_ToLabelsStep : forall index_ind axis df df',
+    df --> df' ->
+    ToLabels index_ind axis df --> ToLabels index_ind axis df'
+| ST_FromLabelsValue : forall axis df df_obj,
+    dfvalue df ->
+    df = DataFrame df_obj ->
+    FromLabels axis df --> DataFrame (Dataframe.FromLabels axis df_obj)
+| ST_FromLabelsStep : forall axis df df',
+    df --> df' ->
+    FromLabels axis df --> FromLabels axis df'
+| ST_ToFromLabels : forall axis df,
+    dfvalue df ->
+    ToLabels 0 axis (FromLabels axis df) --> df
+| ST_MapValues : forall map_func map_dtype axis df df_obj,
+    dfvalue df ->
+    df = DataFrame df_obj ->
+    Map map_func map_dtype axis df --> DataFrame (Dataframe.Map map_func map_dtype axis df_obj)
+| ST_MapStep : forall map_func map_dtype axis df df',
+    df --> df' ->
+    Map map_func map_dtype axis df --> Map map_func map_dtype axis df'
+| ST_ConcatValue : forall concat_type axis other other_obj self self_obj,
+    dfvalue self ->
+    dfvalue other ->
+    self = DataFrame self_obj ->
+    other = DataFrame other_obj ->
+    Concat concat_type axis other self --> DataFrame (Dataframe.Concat concat_type axis other_obj self_obj)
+| ST_ConcatStep : forall concat_type axis other self df,
+    dfvalue self ->
+    dfvalue other ->
+    Concat concat_type axis other self --> df
+| ST_InferDTypesValue : forall axis df df_obj,
+    dfvalue df ->
+    df = DataFrame df_obj ->
+    InferDTypes axis df --> DataFrame (Dataframe.InferDTypes axis df_obj)
+| ST_InferDTypesStep : forall axis df df',
+    df --> df' ->
+    InferDTypes axis df --> InferDTypes axis df'
+                     
+where "t '-->' t'" := (step t t').
+
+Hint Constructors step : core.
+
+(* Define the data typing for operations. *)
+Reserved Notation "'⊢' df '∈' rDT ',' cDT " (at level 40).
+
+Inductive has_dtype : op -> list dtype -> list dtype -> Prop :=
+  | DT_Constructor : forall df_obj,
+      ⊢ (DataFrame df_obj) ∈ (get_row_dtypes df_obj), (get_col_dtypes df_obj)
+  | DT_Transpose : forall df row__dtypes col__dtypes df_obj,
+      ⊢ df ∈ row__dtypes, col__dtypes ->
+      df = DataFrame df_obj ->
+      ⊢ DataFrame (Dataframe.Transpose df_obj) ∈ col__dtypes, row__dtypes
+  | DT_TransposeTwice : forall df row__dtypes col__dtypes df_obj,
+      ⊢ df ∈ row__dtypes, col__dtypes ->
+      df = DataFrame df_obj ->                  
+      ⊢ DataFrame (Dataframe.Transpose (Dataframe.Transpose df_obj)) ∈ row__dtypes, col__dtypes
+  | DT_Mask : forall mask_positions axis df row__dtypes col__dtypes df_obj df_obj',
+      ⊢ df ∈ row__dtypes, col__dtypes ->
+      df = DataFrame df_obj -> 
+      df_obj' = Dataframe.Mask mask_positions axis df_obj ->
+      ⊢ DataFrame df_obj' ∈ (get_row_dtypes df_obj'), (get_col_dtypes df_obj')
+  | DT_Filter : forall filter_func axis df row__dtypes col__dtypes df_obj df_obj',
+      ⊢ df ∈ row__dtypes, col__dtypes ->
+      df = DataFrame df_obj -> 
+      df_obj' = Dataframe.Filter filter_func axis df_obj ->
+      ⊢ DataFrame df_obj' ∈ (get_row_dtypes df_obj'), (get_col_dtypes df_obj')
+  | DT_ToLabels : forall label_ind axis df row__dtypes col__dtypes df_obj df_obj',
+      ⊢ df ∈ row__dtypes, col__dtypes ->
+      df = DataFrame df_obj -> 
+      df_obj' = Dataframe.ToLabels label_ind axis df_obj ->
+      ⊢ DataFrame df_obj' ∈ (get_row_dtypes df_obj'), (get_col_dtypes df_obj')
+  | DT_FromLabels : forall axis df row__dtypes col__dtypes df_obj df_obj',
+      ⊢ df ∈ row__dtypes, col__dtypes ->
+      df = DataFrame df_obj -> 
+      df_obj' = Dataframe.FromLabels axis df_obj ->
+      ⊢ DataFrame df_obj' ∈ (get_row_dtypes df_obj'), (get_col_dtypes df_obj')
+  | DT_Map : forall map_func map_dtypes axis df row__dtypes col__dtypes df_obj df_obj',
+      ⊢ df ∈ row__dtypes, col__dtypes ->
+      df = DataFrame df_obj -> 
+      df_obj' = Dataframe.Map map_func map_dtypes axis df_obj ->
+      ⊢ DataFrame df_obj' ∈ (get_row_dtypes df_obj'), (get_col_dtypes df_obj')
+  | DT_Concat : forall concat_type axis other self other_row__dtypes other_col__dtypes self_row__dtypes self_col__dtypes other_obj self_obj df_obj',
+      ⊢ self ∈ self_row__dtypes, self_col__dtypes ->
+      ⊢ other ∈ other_row__dtypes, other_col__dtypes ->                               
+      self = DataFrame self_obj ->
+      other = DataFrame other_obj ->
+      df_obj' = Dataframe.Concat concat_type axis other_obj self_obj ->
+      ⊢ DataFrame df_obj' ∈ (get_row_dtypes df_obj'), (get_col_dtypes df_obj')
+  | DT_InferDTypes : forall axis df row__dtypes col__dtypes df_obj df_obj',
+      ⊢ df ∈ row__dtypes, col__dtypes ->
+      df = DataFrame df_obj -> 
+      df_obj' = Dataframe.InferDTypes axis df_obj ->
+      ⊢ DataFrame df_obj' ∈ (get_row_dtypes df_obj'), (get_col_dtypes df_obj')
+                                                                                            
+where "'⊢' df '∈' rDT ',' cDT" := (has_dtype df rDT cDT).
+
+Hint Constructors has_dtype : core.
+
+Theorem progress : forall df rDT cDT,
+    ⊢ df ∈ rDT, cDT ->
+                dfvalue df \/ exists df', df --> df'.
+Proof.
+  intros df rDT cDT H.
+  induction H; auto; try (right; destruct IHhas_dtype; destruct H0; eauto).
+Qed.
+  
+Theorem preservation: forall df df' rDT cDT,
+    ⊢ df ∈ rDT, cDT ->
+    df --> df' ->
+    ⊢ df' ∈ rDT, cDT.
+Proof.
+  intros df df' rDT cDT HT HE.
+  generalize dependent df'.
+  induction HT; intros df' HE; try (inversion HE; subst); eauto.
+Qed.
